Semantics/Set.lean
@@ -15,15 +15,15 @@ theorem Set.mem_diff {α : Type u} {s t : Set α} (x : α) :
   ### Basic subset properties
 -/
 
-theorem subset_refl {α : Type} (x : Set α) : x ⊆ x := fun _ => id
+theorem Subset.refl {α : Type} (x : Set α) : x ⊆ x := fun _ => id
 
-theorem subset_trans {α : Type} {x y z : Set α} (h1 : x ⊆ y) (h2 : y ⊆ z) : x ⊆ z :=
+theorem Subset.trans {α : Type} {x y z : Set α} (h1 : x ⊆ y) (h2 : y ⊆ z) : x ⊆ z :=
   fun _ h => h2 (h1 h)
 
-theorem subset_antisymm {α : Type} {x y : Set α} (h1 : x ⊆ y) (h2 : y ⊆ x) : x = y :=
+theorem Subset.antisymm {α : Type} {x y : Set α} (h1 : x ⊆ y) (h2 : y ⊆ x) : x = y :=
   funext fun _ => propext ⟨fun h => h1 h, fun h => h2 h⟩
 
-theorem subset_from_eq {α : Type} {x y : Set α} (h : x = y) : x ⊆ y :=
+theorem Subset.from_eq {α : Type} {x y : Set α} (h : x = y) : x ⊆ y :=
   fun _ h1 => h ▸ h1
 
 /-
@@ -42,32 +42,33 @@ theorem Set.ite_mono (t : Set α) {s₁ s₁' s₂ s₂' : Set α} (h : s₁ ⊆
     | Or.inr h3 => Or.inr ⟨h' h3.1, h3.2⟩
 
 /-
-  ### Set Relations
+  ### Set theoretic (partial) functions
+
+  Really these are just relations, but we can think of them as functions
 -/
 
-namespace SRel
+namespace SFun
 
-notation:20 α " →ᵍ " β => Set (α × β)
+notation:20 α " →ˢ " β => Set (α × β)
 
-def id: α →ᵍ α := {p | p.1 = p.2}
+def id: α →ˢ α := {p | p.1 = p.2}
 
 theorem mem_id:
-  (a, b) ∈ @id α ↔ a = b := Iff.rfl
+  (a, b) ∈ id ↔ a = b := Iff.rfl
 
-def comp (f g: α →ᵍ α): α →ᵍ α :=
+def comp (f g: α →ˢ α): α →ˢ α :=
   {x | ∃z, (x.1, z) ∈ f ∧ (z, x.2) ∈ g}
 
-infixl:90 " ○ " => SRel.comp
+infixl:90 " ○ " => SFun.comp
 
-theorem mem_comp {f g: α →ᵍ α}:
+theorem mem_comp {f g: α →ˢ α}:
   x ∈ f ○ g ↔ ∃z, (x.1, z) ∈ f ∧ (z, x.2) ∈ g := Iff.rfl
 
 theorem comp_mono {α: Type} {f g h k : Set (α × α)}
   (h₁ : f ⊆ h) (h₂ : g ⊆ k): f ○ g ⊆ h ○ k :=
   fun _ ⟨z, h, h'⟩ => ⟨z, h₁ h, h₂ h'⟩
 
-theorem comp_id_right {f: α →ᵍ α}:
-  f ○ id = f := by
+theorem comp_id {f: α →ˢ α}: f ○ id = f := by
   funext x
   apply eq_iff_iff.mpr
   apply Iff.intro
@@ -84,8 +85,7 @@ theorem comp_id_right {f: α →ᵍ α}:
     unfold comp
     exact Exists.intro x.2 (And.intro h rfl)
 
-theorem comp_id_left {f: α →ᵍ α}:
-  id ○ f = f := by
+theorem id_comp {f: α →ˢ α}: id ○ f = f := by
   funext x
   apply eq_iff_iff.mpr
   apply Iff.intro
@@ -102,4 +102,4 @@ theorem comp_id_left {f: α →ᵍ α}:
     unfold comp
     exact Exists.intro x.1 (And.intro rfl h)
 
-end SRel
+end SFun
